Add an induction principle for 'type' which strengthens reasoning for the 'list type' in the Tfunction case; prove 'normalize_type_involutive'

theories/lang/cpp/syntax/types.v
@@ -158,6 +158,62 @@ Inductive type : Set :=
    some Tarch types, like ARM SVE, are "sizeless", hence [option size]. *)
 | Tarch (_ : option bitsize) (name : bs)
 .
+
+Section type_ind'.
+  Variable P : type -> Prop.
+
+  Hypothesis Tptr_ind' : forall (ty : type),
+    P ty -> P (Tptr ty).
+  Hypothesis Tref_ind' : forall (ty : type),
+    P ty -> P (Tref ty).
+  Hypothesis Trv_ref_ind' : forall (ty : type),
+    P ty -> P (Trv_ref ty).
+  Hypothesis Tint_ind' : forall (size : bitsize) (sign : signed),
+    P (Tint size sign).
+  Hypothesis Tvoid_ind' : P Tvoid.
+  Hypothesis Tarray_ind' : forall (ty : type) (sz : N),
+    P ty -> P (Tarray ty sz).
+  Hypothesis Tnamed_ind' : forall (name : globname),
+    P (Tnamed name).
+  Hypothesis Tfunction_ind' : forall {cc : calling_conv} (ty : type) (tys : list type),
+    P ty -> Forall P tys -> P (Tfunction ty tys).
+  Hypothesis Tbool_ind' : P Tbool.
+  Hypothesis Tmember_pointer_ind' : forall (name : globname) (ty : type),
+    P ty -> P (Tmember_pointer name ty).
+  Hypothesis Tfloat_ind' : forall (size : bitsize),
+    P (Tfloat size).
+  Hypothesis Tqualified_ind' : forall (q : type_qualifiers) (ty : type),
+    P ty -> P (Tqualified q ty).
+  Hypothesis Tnullptr_ind' : P Tnullptr.
+  Hypothesis Tarch_ind' : forall (osize : option bitsize) (name : bs),
+    P (Tarch osize name).
+
+  Fixpoint type_ind' (ty : type) : P ty :=
+    match ty with
+    | Tptr ty                 => Tptr_ind' ty (type_ind' ty)
+    | Tref ty                 => Tref_ind' ty (type_ind' ty)
+    | Trv_ref ty              => Trv_ref_ind' ty (type_ind' ty)
+    | Tint sz sgn             => Tint_ind' sz sgn
+    | Tvoid                   => Tvoid_ind'
+    | Tarray ty sz            => Tarray_ind' ty sz (type_ind' ty)
+    | Tnamed name             => Tnamed_ind' name
+    | Tfunction ty tys        =>
+      Tfunction_ind' ty tys (type_ind' ty)
+                     ((fix list_tys_ind' (tys : list type) : Forall P tys :=
+                         match tys with
+                         | []        => List.Forall_nil P
+                         | ty :: tys' => List.Forall_cons P ty tys'
+                                                        (type_ind' ty) (list_tys_ind' tys')
+                         end) tys)
+    | Tbool                   => Tbool_ind'
+    | Tmember_pointer name ty => Tmember_pointer_ind' name ty (type_ind' ty)
+    | Tfloat sz               => Tfloat_ind' sz
+    | Tqualified q ty         => Tqualified_ind' q ty (type_ind' ty)
+    | Tnullptr                => Tnullptr_ind'
+    | Tarch osize name        => Tarch_ind' osize name
+    end.
+End type_ind'.
+
 Notation Tchar := Tint (only parsing).
 (* XXX merge type_eq_dec into type_eq. *)
 Definition type_eq_dec : forall (ty1 ty2 : type), { ty1 = ty2 } + { ty1 <> ty2 }.
@@ -323,6 +379,63 @@ Fixpoint normalize_type (t : type) : type :=
   | Tfloat _ => t
   | Tarch _ _ => t
   end.
+
+Section normalize_type_involutive.
+  Lemma merge_tq_assoc:
+    forall q q' q'',
+      merge_tq q (merge_tq q' q'') = merge_tq (merge_tq q q') q''.
+  Proof. now intros *; rewrite /merge_tq/= !orb_assoc. Qed.
+
+  Lemma type_Tqualified_dec:
+    forall ty,
+      {exists q ty', ty = Tqualified q ty'} + {not(exists q ty', ty = Tqualified q ty')}.
+  Proof.
+    intros *; destruct ty;
+      try solve[apply right; intros [? [? CONTRA]]; inversion CONTRA].
+    apply left; eauto.
+  Qed.
+
+  Fixpoint _drop_norm_involutive q q' ty {struct ty}:
+    qual_norm' (fun _ t => normalize_type t) q (qual_norm' (fun _ t => normalize_type t) q' ty) =
+    qual_norm' (fun _ t => normalize_type t) (merge_tq q q') ty
+  with _qual_norm_involutive q ty {struct ty}:
+    normalize_type (qual_norm' (fun q t => tqualified q (normalize_type t)) q ty) =
+    qual_norm' (fun q t => tqualified q (normalize_type t)) q ty
+  with normalize_type_involutive ty {struct ty}:
+    normalize_type (normalize_type ty) = normalize_type ty.
+  Proof.
+    { (* _drop_norm_involutive *)
+      generalize dependent q; generalize dependent q';
+        induction ty using type_ind'; intros *;
+        rewrite /qual_norm/= ?normalize_type_involutive//.
+      - rewrite map_map /qual_norm !IHty /merge_tq/=;
+          erewrite map_ext_Forall; eauto; eapply Forall_impl; eauto;
+          intros * HForall; simpl in HForall; apply HForall.
+      - now rewrite IHty merge_tq_assoc.
+    }
+    { (* _qual_norm_involutive *)
+      intros *; generalize dependent q;
+        induction ty using type_ind'; intros *; simpl;
+        try solve[destruct q as [[|] [|]]; simpl; now rewrite ?normalize_type_involutive].
+      destruct q as [[|] [|]]; simpl;
+        rewrite map_map /qual_norm ?_drop_norm_involutive /merge_tq/=;
+        try solve[erewrite map_ext_Forall; eauto; induction tys;
+                  [ now constructor
+                  | constructor;
+                    [ now apply _drop_norm_involutive
+                    | apply IHtys; now apply Forall_inv_tail in H]]].
+    }
+    {
+      intros *; induction ty using type_ind'; simpl; rewrite ?IHty; eauto.
+      rewrite map_map /qual_norm _drop_norm_involutive /merge_tq/=.
+      erewrite map_ext_Forall; eauto; induction tys;
+        [ now constructor
+        | constructor;
+          [ now apply _drop_norm_involutive
+          | apply IHtys; now apply Forall_inv_tail in H]].
+    }
+  Qed.
+End normalize_type_involutive.
 
 Definition decompose_type : type -> type_qualifiers * type :=
   qual_norm (fun q t => (q, t)).
